\section{Lecture 8 -- 5th November 2024}\label{sec: lecture 8}
We continue towards our proof of the prime number theorem by estimating the ratio $\frac{\vartheta(x)}{x}$. 
\begin{lemma}\label{lem: boundedness of theta function ratio}
    The function $\frac{\vartheta(x)}{x}$ is bounded on $[1,\infty)$. 
\end{lemma}
\begin{proof}
    Consider the binomial coefficient $\binom{2k}{k}$. Let $k$ be a postive integer. If $k<p<2k$, then $p|\binom{2k}{k}$ since writing the factorial as 
    $$\binom{2k}{k}=\frac{(2k)\dots(k+1)}{k!}$$
    we have that $p$ is in the numerator, but not canceled out by the denominator as $p$ is prime. In particular, this holds for each $p$ for $k<p<2k$ so we have 
    $$\prod_{k<p<2k}p\leq\binom{2k}{k}\leq 2^{2k}$$
    where the second inequality follows from $\sum_{r=0}^{2k}\binom{2k}{r}=2^{2k}$. Passing to the logarithm, we have 
    $$\sum_{k<p\leq 2k}\log(p)\leq 2k\cdot\log(2).$$
    Taking $k=2^{\ell-1}$ for some $\ell$, we obtain 
    $$\sum_{p\leq 2^{\ell}}\log(p)\leq2^{\ell+1}\log(2)$$
    by summing inequalities of the above form. Noting for any $x\in\RR_{\geq0}$ an $\ell$ such that $2^{\ell-1}<x\leq 2^{\ell}$ we have 
    \begin{align*}
        \vartheta(x) &\leq \sum_{p\leq 2^{\ell}}\log(p) \\
        &\leq 2^{\ell+1}\log(2) \\
        &\leq 4x\log(2)
    \end{align*}
    giving $\frac{\vartheta(x)}{x}\leq 4\log(2)$ hence the claim. 
\end{proof}
Recalling the construction of the Mellin transform from \Cref{def: Mellin transform}, we show the following. 
\begin{lemma}\label{lem: mellin tranfsormation of theta function}
    The Mellin transform $\Mcal_{\vartheta(x)}(s)$ of the Theta function $\vartheta(x)$ is given by 
    $$\Mcal_{\vartheta(x)}(s)=\sum_{p\text{ prime}}\frac{\log(p)}{p^{s}}=-\frac{\zeta'(s)}{\zeta(s)}-\sum_{p\text{ prime}}\frac{\log(p)}{p^{s}(p^{s}-1)}$$
    for $\RE(s)>1$. 
\end{lemma}
\begin{proof}
    We compute 
    \begin{align*}
        \Mcal_{\vartheta(x)}(s)&=s\int_{1}^{\infty}\vartheta(x)x^{-s-1}dx \\
        &= \sum_{n=1}^{\infty}s\int_{n}^{n+1}\vartheta(x)x^{-s-1}dx && \vartheta\text{ constant on interval}\\
        &= \sum_{n=1}^{\infty}s\vartheta(n)\int_{n}^{n+1}x^{-s-1}dx && \vartheta(x)=\vartheta(n)\text{ on interval }[n,n+1] \\
        &= \sum_{n=1}^{\infty}s\vartheta(n)\left(\frac{x^{-s}}{-s}|_{s=n}^{n+1}\right) \\
        &= \sum_{n=1}^{\infty}\vartheta(n)\left(n^{-s}-(n+1)^{-s}\right)
    \end{align*}
    where we note this is convergent for $\RE(s)>1$. Taking $\RE(s)>2$ we can decompose the sum 
    \begin{align*}
        &=\sum_{n=1}^{\infty}\vartheta(n)n^{-s} - \sum_{n=1}^{\infty}\vartheta(n)(n+1)^{-s} \\ 
        &=\sum_{n=1}^{\infty}\vartheta(n)n^{-s} - \sum_{n=2}^{\infty}\vartheta(n-1)n^{-s} && \text{changing index of summation in 2nd sum} \\
        &= \sum_{n=1}^{\infty}(\vartheta(n)-\vartheta(n-1))n^{-s}
    \end{align*}
    but noting
    $$\vartheta(n)-\vartheta(n-1)=\begin{cases}
        \log(n) & n \text{ prime}\\
        0 & \text{otherwise}
    \end{cases}$$
    the above expression simplifies to $\sum_{p\text{ prime}}\frac{\log(p)}{p^{s}}$. Since this also converges for $\RE(s)>1$, the identity theorem \Cref{thm: identity theorem} allows us to extend this function to agree with $\Mcal_{\vartheta(x)}(s)$ on this halfspace. 
    
    For the second equality, we consider the logarithmic derivative of $\zeta(s)$ as an Euler product in \Cref{thm: zeta function by infinite products} to observe 
    \begin{align*}
        -\frac{\zeta'(s)}{\zeta(s)} &= \sum_{p\text{ prime}}\frac{p^{-s}\log(p)}{1-p^{-s}} \\
        &= \sum_{p\text{ prime}}\frac{\log(p)}{p^{s}-1}
    \end{align*}
    with 
    $$\sum_{p\text{ prime}}\frac{\log(p)}{p^{s}-1}-\sum_{p\text{ prime}}\frac{\log(p)}{p^{s}(p^{s}-1)}=\sum_{p\text{ prime}}\frac{\log(p)}{p^{s}}$$
    giving the claim. 
\end{proof}
In summary, we have the following. 
\begin{proposition}\label{prop: Mellin transform of theta function minus x}
    The Mellin transform $\Mcal_{\vartheta(x)-x}(s)$ of the function $\vartheta(x)-x$ is given by 
    \begin{equation*}\label{eqn: Mellin transformation of theta x minus x}
        \Mcal_{\vartheta(x)-x}(s)=-\frac{\zeta'(s)}{\zeta(s)}-1-\frac{1}{s-1}-\sum_{p\text{ prime}}\frac{\log(p)}{p^{s}(p^{s}-1)}
    \end{equation*}
    for $\RE(s)>1$. 
\end{proposition}
\begin{proof}
    This follows from \Cref{lem: Mellin transform of x} and the second equality of \Cref{lem: mellin tranfsormation of theta function}. 
\end{proof}
The summation term of (\ref{eqn: Mellin transformation of theta x minus x}) converges for $\RE(s)>\frac{1}{2}$ and the pole of $\zeta(s)$ at $s=1$ of order 1 to be negated by the sum with the Mellin transform of $x$, suggesting that the function can be extended holomorphically to a neighborhood of the closed halfspace. To conclude the proof of the prime number theorem, we will provide an estimate of this function by extending the domain of definition for the Mellin transform to the closed halfspace $\RE(s)\geq 1$. 